To separate the state into a tensor product of two single-qubit states, we need to represent it in the following way:

$$
\begin{bmatrix} \alpha \gamma \\\ \alpha \delta \\\ \beta \gamma \\\ \beta \delta \end{bmatrix} = 
\begin{bmatrix} \alpha \\\ \beta \end{bmatrix} \otimes \begin{bmatrix} \gamma \\\ \delta \end{bmatrix}
$$

This brings us to a system of equations:

$$
\begin{cases}
\alpha\gamma = \frac{1}{2} \\\ \alpha\delta = \frac{i}{2} \\\ \beta \gamma = \frac{-i}{2} \\\ \beta \delta = \frac{1}{2}
\end{cases}
$$

Solving this system of equations gives us the answer:

$$\alpha = \frac{1}{\sqrt2}, \beta = \frac{-i}{\sqrt2}, \gamma = \frac{1}{\sqrt2}, \delta = \frac{i}{\sqrt2}$$

$$
\frac{1}{2} \begin{bmatrix} 1 \\\ i \\\ -i \\\ 1 \end{bmatrix} =
\frac{1}{\sqrt2} \begin{bmatrix} 1 \\\ -i \end{bmatrix} \otimes \frac{1}{\sqrt2} \begin{bmatrix} 1 \\\ i \end{bmatrix}
$$


> Note that finding such representation is not always possible, as you will see in the next exercise.
